# Project Report
# random
g = 0:
$$
\begin{split}
cdf(x) &= \int^x_{\alpha_0}\frac{\eta_0}{(\alpha_0^{-\eta_0}-\beta_0^{-\eta_0})}\times t^{-\eta_0-1}dt \\
&=\frac{\eta_0}{\alpha_0^{-\eta_0}-\beta_0^{-\eta_0}}\times\frac{1}{-\eta_0}\times t^{-\eta_0}\mid^x_{\alpha_0}\\
&=\frac{\alpha^{-\eta_0}-x^{-\eta_0}}{\alpha_0^{-\eta_0}-\beta_0^{-\eta_0}}\\
icdf(x)&=\sqrt[-\eta_0]{\alpha_0^{-\eta_0}-(\alpha_0^{-\eta_0}-\beta_0^{-\eta_0})\times x}, x\in U[0,1]

\end{split}
$$
g=1:
$$
\begin{split}
cdf(x) &= \int^x_{\alpha_1}\frac{\eta_1}{\alpha_1^{-\eta_1}}\times t^{-\eta_1-1}dt \\ 
&=\frac{\eta_1}{\alpha_1^{-\eta_1}}\times \frac{1}{-\eta_1}\times t^{-\eta_1}\mid^x_{\alpha_1}\\
&=1-\frac{x^{-\eta_1}}{\alpha_1^{-\eta_1}}\\
icdf(x)&=\sqrt[-\eta_1]{1-x}\times\alpha_1^{-\eta_1},x\in U[0,1]


\end{split}
$$
